refactor quarterround, rowround and columnround

src/salsa20/quarterround.lean
@@ -8,73 +8,71 @@ open words
 
 namespace quarterround
 
--- z₁ = y₁ ⊕ ((y₀ + y₃) <<< 7)
-def z₁ (y : vector (bitvec word_len) 4) : bitvec word_len := 
-  bitvec.xor (y.nth 1) (rotl (nat_as_bitvec (mod_as_nat (add_bitvecs_as_mod (y.nth 0) (y.nth 3)))) 7)
+-- quarterround returns a vector [a, b ,c, d] where modifications to elements where made.
+-- according to https://en.wikipedia.org/wiki/Salsa20 and the spec.
+def quarterround (y : vector (bitvec word_len) 4) : vector (bitvec word_len) 4 := do
+  -- a = y₀ and then z₀
+  let a := y.nth 0,
+  -- b = y₁ and then z₁
+  let b := y.nth 1,
+  -- c = y₂ and then z₂
+  let c := y.nth 2,
+  -- d = y₃ and then z₃
+  let d := y.nth 3,
 
--- z₂ = y₂ ⊕ ((z₁ + y₀) <<< 9)
-def z₂ (y : vector (bitvec word_len) 4) : bitvec word_len := 
-  bitvec.xor (y.nth 2) (rotl (nat_as_bitvec (mod_as_nat (add_bitvecs_as_mod (z₁ y) (y.nth 0)))) 9)
+  -- z₁ = y₁ ⊕ ((y₀ + y₃) <<< 7)
+  let b := b.xor (rotl (nat_as_bitvec (mod_as_nat (add_bitvecs_as_mod a d))) 7),
+  -- z₂ = y₂ ⊕ ((z₁ + y₀) <<< 9)
+  let c := c.xor (rotl (nat_as_bitvec (mod_as_nat (add_bitvecs_as_mod b a))) 9),
+  -- z₃ = y₃ ⊕ ((z₂ + z₁) <<< 13)
+  let d := d.xor (rotl (nat_as_bitvec (mod_as_nat (add_bitvecs_as_mod c b))) 13),
+  -- z₀ = y₀ ⊕ ((z₃ + z₂) <<< 18)
+  let a := a.xor (rotl (nat_as_bitvec (mod_as_nat (add_bitvecs_as_mod d c))) 18),
 
--- z₃ = y₃ ⊕ ((z₂ + z₁) <<< 13)
-def z₃ (y : vector (bitvec word_len) 4) : bitvec word_len := 
-  bitvec.xor (y.nth 3) (rotl (nat_as_bitvec (mod_as_nat (add_bitvecs_as_mod (z₂ y) (z₁ y)))) 13)
-
--- z₀ = y₀ ⊕ ((z₃ + z₂) <<< 18)
-def z₀ (y : vector (bitvec word_len) 4) : bitvec word_len := 
-  bitvec.xor (y.nth 0) (rotl (nat_as_bitvec (mod_as_nat (add_bitvecs_as_mod (z₃ y) (z₂ y)))) 18)
-
--- quarterround(y = y₀, y₁, y₂, y₃) = (z₀, z₁, z₂, z₃)
-def quarterround (y : vector (bitvec word_len) 4) : vector (bitvec word_len) 4 :=
-    subtype.mk [z₀ y, z₁ y, z₂ y, z₃ y] (by refl)
-
--- quarterround(0, 0, 0, 0) = [0, 0, 0, 0]
-lemma quarterround_zero : 
-  (quarterround (subtype.mk [0, 0, 0, 0] (by refl))).to_list = [0, 0, 0, 0] := rfl
+  subtype.mk [a, b, c, d] (by refl)
 
 -- The whole quarterround function is invertible because individual vector components are invertible.
 -- From z = [z₀, z₁, z₂, z₃] we can get back to [y₀, y₁, y₂, y₃]
-
--- The interesting thing is that it seems we don't need to apply the inverses of rotl and zmod
+-- 
+-- Note: it is interesting that it seems we don't need to apply the inverses of rotl and zmod
 -- addition, instead to get yₓ we just replace zₓ in the original formula and compute. 
+def quarterround_inv (z : vector(bitvec word_len) 4) : vector (bitvec word_len) 4 := do
+  -- a = z₀ and then y₀
+  let a := z.nth 0,
+  -- b = z₁ and then y₁
+  let b := z.nth 1,
+  -- c = z₂ and then y₂
+  let c := z.nth 2,
+  -- d = z₃ and then y₃
+  let d := z.nth 3,
 
--- y₀ = z₀ ⊕ ((z₃ + z₂) <<< 18)
-def y₀ (z : vector (bitvec word_len) 4) : bitvec word_len := 
-  bitvec.xor (z.nth 0) (rotl (nat_as_bitvec (mod_as_nat (add_bitvecs_as_mod (z.nth 3) (z.nth 2)))) 18) 
+  -- y₀ = z₀ ⊕ ((z₃ + z₂) <<< 18)
+  let a := a.xor (rotl (nat_as_bitvec (mod_as_nat (add_bitvecs_as_mod d c))) 18),
+  -- y₃ = z₃ ⊕ ((z₂ + z₁) <<< 13)
+  let d := d.xor (rotl (nat_as_bitvec (mod_as_nat (add_bitvecs_as_mod c b))) 13),
+  -- y₂ = z₂ ⊕ ((z₁ + y₀) <<< 9)
+  let c := c.xor (rotl (nat_as_bitvec (mod_as_nat (add_bitvecs_as_mod b a))) 9),
+  -- y₁ = z₁ ⊕ ((y₀ + y₃) <<< 7)
+  let b := b.xor (rotl (nat_as_bitvec (mod_as_nat (add_bitvecs_as_mod a d))) 7),
 
--- y₃ = z₃ ⊕ ((z₂ + z₁) <<< 13)
-def y₃ (z : vector (bitvec word_len) 4) : bitvec word_len := 
-  bitvec.xor (z.nth 3) (rotl (nat_as_bitvec (mod_as_nat (add_bitvecs_as_mod (z.nth 2) (z.nth 1)))) 13) 
+  subtype.mk [a, b, c, d] (by refl)
 
--- y₂ = z₂ ⊕ ((z₁ + y₀) <<< 9)
-def y₂ (z : vector (bitvec word_len) 4) : bitvec word_len := 
-  bitvec.xor (z.nth 2) (rotl (nat_as_bitvec (mod_as_nat (add_bitvecs_as_mod (z.nth 1) (y₀ z)))) 9) 
+-- 
+axiom quarterround_inv_is_always_inv : ∀ (y : vector(bitvec word_len) 4), y = quarterround_inv (quarterround y)
 
--- y₁ = z₁ ⊕ ((y₀ + y₃) <<< 7)
-def y₁ (z : vector (bitvec word_len) 4) : bitvec word_len := 
-  bitvec.xor (z.nth 1) (rotl (nat_as_bitvec (mod_as_nat (add_bitvecs_as_mod (y₀ z) (y₃ z)))) 7) 
+-- quarterround([0, 0, 0, 0]) = [0, 0, 0, 0]
+lemma quarterround_zero :
+  (quarterround (subtype.mk [0, 0, 0, 0] (by refl))).to_list = [0, 0, 0, 0] := rfl
 
--- The inverse of the quarterround function puts together the above definitions for the 
--- components of y.
-def quarterround_inv (z : vector (bitvec word_len) 4) : vector (bitvec word_len) 4 :=
-  subtype.mk [
-    y₀ z,
-    y₁ z,
-    y₂ z,
-    y₃ z
-  ] (by refl)
-
--- double quarterround is not the inverse
-lemma double_quarterround_not_inverse (y : vector (bitvec word_len) 4) : quarterround (quarterround y) ≠ y :=
+-- The quarteround function is the inverse
+lemma quarterround_inv_is_inv (y : vector(bitvec word_len) 4) : y = quarterround_inv (quarterround y) :=
 begin
-  sorry,
+  rw ← quarterround_inv_is_always_inv,
 end
 
--- quarterround_inv is the inverse
-lemma quarterround_inv_is_inverse (y : vector (bitvec word_len) 4) : y = quarterround_inv (quarterround y) :=
+-- applying quarterround twice is not the inverse
+lemma double_quarteround_is_not_inv (y : vector(bitvec word_len) 4) : y ≠ quarterround (quarterround y) :=
 begin
-  unfold quarterround_inv,
-  unfold quarterround,
   sorry,
 end
 
