src/salsa20/columnround.lean
@@ -2,71 +2,46 @@
   Section 5 : The columnrow function
   http://cr.yp.to/snuffle/spec.pdf
 -/
+import data.matrix.basic
+
 import salsa20.words
 import salsa20.quarterround
+import salsa20.rowround
 
 open words
 open quarterround
+open rowround
 
 namespace columnround
 
--- (y₀, y₄, y₈, y₁₂) = quarterround(x₀, x₄, x₈, x₁₂)
-def columnround1 (x₀ x₄ x₈ x₁₂ : bitvec word_len) : vector (bitvec word_len) 4 := 
-  quarterround (subtype.mk [x₀, x₄, x₈, x₁₂] (by refl))
+-- Given a 4x4 matrix convert it to a vector of 16 word bitvects.
+def matrix_as_vector (Y : matrix (fin 4) (fin 4) (bitvec word_len)) : vector (bitvec word_len) 16 :=
+  subtype.mk [
+    Y 0 0, Y 0 1, Y 0 2, Y 0 3,
+    Y 1 0, Y 1 1, Y 1 2, Y 1 3,
+    Y 2 0, Y 2 1, Y 2 2, Y 2 3,
+    Y 3 0, Y 3 1, Y 3 2, Y 3 3
+  ] (by refl)
 
--- (y₅, y₉, y₁₃, y₁) = quarterround(x₅, x₉, x₁₃, x₁)
-def columnround2 (x₅ x₉ x₁₃ x₁ : bitvec word_len) : vector (bitvec word_len) 4 := 
-  quarterround (subtype.mk [x₅, x₉, x₁₃, x₁] (by refl))
+-- The columnround function defined as the transpose of the rowround
+def columnround (y : vector(bitvec word_len) 16) : matrix (fin 4) (fin 4) (bitvec word_len) := do
+  -- transpose the input
+  let Y := (vector_as_matrix y).transpose,
+  -- apply rowround and transpose the result
+  (rowround (matrix_as_vector Y)).transpose
 
--- (y₁₀, y₁₄, y₂, y₆) = quarterround(x₁₀, x₁₄, x₂, x₆)
-def columnround3 (x₁₀ x₁₄ x₂ x₆ : bitvec word_len) : vector (bitvec word_len) 4 := 
-  quarterround (subtype.mk [x₁₀, x₁₄, x₂, x₆] (by refl))
-
--- (y₁₅, y₃, y₇, y₁₁) = quarterround(x₁₅, x₃, x₇, x₁₁)
-def columnround4 (x₁₅ x₃ x₇ x₁₁ : bitvec word_len) : vector (bitvec word_len) 4 := 
-  quarterround (subtype.mk [x₁₅, x₃, x₇, x₁₁] (by refl))
-
--- If x = (x₀, x₁, x₂, x₃, ... , x₁₅) then 
--- columnround(x) = (y₀, y₁, y₂, y₃, ... , y₁₅) where
--- (y₀, y₄, y₈, y₁₂) = quarterround(x₀, x₄, x₈, x₁₂)
--- (y₅, y₉, y₁₃, y₁) = quarterround(x₅, x₉, x₁₃, x₁)
--- (y₁₀, y₁₄, y₂, y₆) = quarterround(x₁₀, x₁₄, x₂, x₆)
--- (y₁₅, y₃, y₇, y₁₁) = quarterround(x₁₅, x₃, x₇, x₁₁)
-def columnround
-  (x : vector (bitvec word_len) 16) : vector (bitvec word_len) 16 :=
-  do
-    let c1 := columnround1 (x.nth 0) (x.nth 4) (x.nth 8) (x.nth 12),
-    let c2 := columnround2 (x.nth 5) (x.nth 9) (x.nth 13) (x.nth 1),
-    let c3 := columnround3 (x.nth 10) (x.nth 14) (x.nth 2) (x.nth 6),
-    let c4 := columnround4 (x.nth 15) (x.nth 3) (x.nth 7) (x.nth 11),
-
-    let y₀ := c1.head,
-    let y₄ := c1.nth 1,
-    let y₈ := c1.nth 2,
-    let y₁₂ := c1.nth 3,
-
-    let y₅ := c2.head,
-    let y₉ := c2.nth 1,
-    let y₁₃ := c2.nth 2,
-    let y₁ := c2.nth 3,
-
-    let y₁₀ := c3.head,
-    let y₁₄ := c3.nth 1,
-    let y₂ := c3.nth 2,
-    let y₆ := c3.nth 3,
-
-    let y₁₅ := c4.head,
-    let y₃ := c4.nth 1,
-    let y₇ := c4.nth 2,
-    let y₁₁ := c4.nth 3,
-
-    subtype.mk [y₀, y₁, y₂, y₃, y₄, y₅, y₆, y₇, y₈, y₉, y₁₀, y₁₁, y₁₂, y₁₃, y₁₄, y₁₅] (by refl)
-
+-- The columnround of input all zeros is a matrix where its componenets are all zeros.
 lemma columnround_zero : 
   columnround (subtype.mk [0, 0, 0, 0, 0, 0, 0, 0, 0, 0, 0, 0, 0, 0, 0, 0] (by refl)) = 
-    subtype.mk [0, 0, 0 ,0, 0, 0, 0, 0, 0, 0, 0, 0 ,0 ,0, 0, 0] (by refl) := rfl
+    ![
+     ![0, 0, 0 ,0],
+     ![0, 0, 0 ,0],
+     ![0, 0, 0 ,0],
+     ![0, 0, 0 ,0]
+    ] :=
+    begin
+      exact dec_trivial,
+    end
 
--- TODO: equivalent formula
--- TODO: matrix form
 
 end columnround
