src/salsa20/rowround.lean
@@ -2,69 +2,59 @@
   Section 4 : The rowround function
   http://cr.yp.to/snuffle/spec.pdf
 -/
+import data.matrix.basic
+
 import salsa20.words
 import salsa20.quarterround
+
+open matrix
 
 open words
 open quarterround
 
 namespace rowround
 
--- (z₀, z₁, z₂, z₃) = quarterround(y₀, y₁, y₂, y₃)
-def rowround1 (y₀ y₁ y₂ y₃ : bitvec word_len) : vector (bitvec word_len) 4 := 
-  quarterround (subtype.mk [y₀, y₁, y₂, y₃] (by refl))
+-- Given a vector of 16 words, convert it to a 4x4 matrix.
+def vector_as_matrix (y : vector(bitvec word_len) 16) : matrix (fin 4) (fin 4) (bitvec word_len) :=
+  ![
+    ![(y.nth 0), (y.nth 1), (y.nth 2), (y.nth 3)],
+    ![(y.nth 4), (y.nth 5), (y.nth 6), (y.nth 7)],
+    ![(y.nth 8), (y.nth 9), (y.nth 10), (y.nth 11)],
+    ![(y.nth 12), (y.nth 13), (y.nth 14), (y.nth 15)]
+  ]
 
--- (z₅, z₆, z₇, z₄) = quarterround(y₅, y₆, y₇, y₄)
-def rowround2 (y₅ y₆ y₇ y₄ : bitvec word_len) : vector (bitvec word_len) 4 := 
-  quarterround (subtype.mk [y₅, y₆, y₇, y₄] (by refl))
+-- The rowround function in the matrix form
+def rowround (y : vector(bitvec word_len) 16) : matrix (fin 4) (fin 4) (bitvec word_len) := do
+  let Y := vector_as_matrix y,
 
--- (z₁₀, z₁₁, z₈, z₉) = quarterround(y₁₀, y₁₁, y₈, y₉)
-def rowround3 (y₁₀ y₁₁ y₈ y₉ : bitvec word_len) : vector (bitvec word_len) 4 := 
-  quarterround (subtype.mk [y₁₀, y₁₁, y₈, y₉] (by refl))
+  -- (z₀, z₁, z₂, z₃) = quarterround(y₀, y₁, y₂, y₃)
+  let row1 := quarterround (subtype.mk [(Y 0 0), (Y 0 1), (Y 0 2), (Y 0 3)] (by refl)),
+  -- (z₅, z₆, z₇, z₄) = quarterround(y₅, y₆, y₇, y₄)
+  let row2 := quarterround (subtype.mk [(Y 1 1), (Y 1 2), (Y 1 3), (Y 1 0)] (by refl)),
+  -- (z₁₀, z₁₁, z₈, z₉) = quarterround(y₁₀, y₁₁, y₈, y₉)
+  let row3 := quarterround (subtype.mk [(Y 2 2), (Y 2 3), (Y 2 0), (Y 2 1)] (by refl)),
+  -- quarterround(y₁₅, y₁₂, y₁₃, y₁₄)
+  let row4 := quarterround (subtype.mk [(Y 3 3), (Y 3 0), (Y 3 1), (Y 3 2)] (by refl)),
 
--- (z₁₅, z₁₂, z₁₃, z₁₄) = quarterround(y₁₅, y₁₂, y₁₃, y₁₄)
-def rowround4 (y₁₅ y₁₂ y₁₃ y₁₄ : bitvec word_len) : vector (bitvec word_len) 4 := 
-  quarterround (subtype.mk  [y₁₅, y₁₂, y₁₃, y₁₄] (by refl))
+  let new_matrix := 
+  ![
+    ![(row1.nth 0), (row1.nth 1), (row1.nth 2), (row1.nth 3)],
+    ![(row2.nth 3), (row2.nth 0), (row2.nth 1), (row2.nth 2)],
+    ![(row3.nth 2), (row3.nth 3), (row3.nth 0), (row3.nth 1)],
+    ![(row4.nth 1), (row4.nth 2), (row4.nth 3), (row4.nth 0)]
+  ],
 
--- If y = (y₀, y₁, y₂, y₃, ... , y₁₅) then 
--- rowround(y) = (z₀, z₁, z₂, z₃, ... , z₁₅) where
--- (z₀, z₁, z₂, z₃) = quarterround(y₀, y₁, y₂, y₃)
--- (z₅, z₆, z₇, z₄) = quarterround(y₅, y₆, y₇, y₄)
--- (z₁₀, z₁₁, z₈, z₉) = quarterround(y₁₀, y₁₁, y₈, y₉)
--- (z₁₅, z₁₂, z₁₃, z₁₄) = quarterround(y₁₅, y₁₂, y₁₃, y₁₄)
-def rowround (y : vector(bitvec word_len) 16) : vector (bitvec word_len) 16 :=
-  do
-    let r1 := rowround1 (y.nth 0) (y.nth 1) (y.nth 2) (y.nth 3),
-    let r2 := rowround2 (y.nth 5) (y.nth 6) (y.nth 7) (y.nth 4),
-    let r3 := rowround3 (y.nth 10) (y.nth 11) (y.nth 8) (y.nth 9),
-    let r4 := rowround4 (y.nth 15) (y.nth 12) (y.nth 13) (y.nth 14),
+  new_matrix
 
-    let z₀ := r1.head,
-    let z₁ := r1.nth 1,
-    let z₂ := r1.nth 2,
-    let z₃ := r1.nth 3,
-
-    let z₅ := r2.head,
-    let z₆ := r2.nth 1,
-    let z₇ := r2.nth 2,
-    let z₄ := r2.nth 3,
-
-    let z₁₀ := r3.head,
-    let z₁₁ := r3.nth 1,
-    let z₈ := r3.nth 2,
-    let z₉ := r3.nth 3,
-
-    let z₁₅ := r4.head,
-    let z₁₂ := r4.nth 1,
-    let z₁₃ := r4.nth 2,
-    let z₁₄ := r4.nth 3,
-
-    subtype.mk [z₀, z₁, z₂, z₃, z₄, z₅, z₆, z₇, z₈, z₉, z₁₀, z₁₁, z₁₂, z₁₃, z₁₄, z₁₅] (by refl)
-
-lemma rowround_zero : 
+-- The rowround of input all zeros is a matrix where its componenets are all zeros.
+lemma rowround_zero :
   rowround (subtype.mk [0, 0, 0, 0, 0, 0, 0, 0, 0, 0, 0, 0, 0, 0, 0, 0] (by refl)) = 
-    subtype.mk  [0, 0, 0 ,0, 0, 0, 0, 0, 0, 0, 0, 0 ,0 ,0, 0, 0] (by refl) := rfl
+    ![
+     ![0, 0, 0 ,0],
+     ![0, 0, 0 ,0],
+     ![0, 0, 0 ,0],
+     ![0, 0, 0 ,0]
+    ] := rfl
 
--- TODO: matrix form
 
 end rowround
